Fix tailcalls

backend/Asmgenproof0.v
@@ -1068,10 +1068,11 @@ Section MATCH_STACK.
 Variable ge: Mach.genv.
 Variable m: mem.
 
-Inductive match_stack: list Mach.stackframe -> Prop :=
-  | match_stack_nil:
-      match_stack nil
-  | match_stack_cons: forall fb sg sp ra c s f tf tc dra dsp bsp osp,
+Inductive match_stack: signature -> list Mach.stackframe -> Prop :=
+  | match_stack_nil: forall sg,
+      sig_res sg = sig_res signature_main ->
+      match_stack sg nil
+  | match_stack_cons: forall sg' fb sg sp ra c s f tf tc dra dsp bsp osp,
       Genv.find_funct_ptr ge fb = Some (Internal f) ->
       forall (TAIL: is_tail c (Mach.fn_code f)),
       transl_code_at_pc ge (Vptr fb ra) fb f c false tf tc ->
@@ -1079,17 +1080,18 @@ Inductive match_stack: list Mach.stackframe -> Prop :=
       forall (COMP_SP: Mem.val_compartment m sp = comp_of f),
       forall (SP: sp = Vptr bsp osp),
       forall (SP_VALID: Mem.valid_block m bsp),
-      match_stack s ->
-      match_stack (Mach.Stackframe fb sg sp ra c dra dsp :: s).
+      forall (LOC_RES: sig_res sg' = sig_res sg),
+      match_stack (Mach.fn_sig f) s ->
+      match_stack sg' (Mach.Stackframe fb sg sp ra c dra dsp :: s).
 
-Lemma parent_sp_def: forall s, match_stack s -> dummy_parent_sp s <> Vundef.
+Lemma parent_sp_def: forall sg s, match_stack sg s -> dummy_parent_sp s <> Vundef.
 Proof.
   induction 1; simpl.
   unfold Vnullptr; destruct Archi.ptr64; congruence.
   destruct dsp; auto. discriminate.
 Qed.
 
-Lemma parent_ra_def: forall s, match_stack s -> dummy_parent_ra s <> Vundef.
+Lemma parent_ra_def: forall sg s, match_stack sg s -> dummy_parent_ra s <> Vundef.
 Proof.
   induction 1; simpl.
   unfold Vnullptr; destruct Archi.ptr64; congruence.
@@ -1097,15 +1099,15 @@ Proof.
 Qed.
 
 Lemma lessdef_parent_sp:
-  forall s v,
-  match_stack s -> Val.lessdef (dummy_parent_sp s) v -> v = dummy_parent_sp s.
+  forall sg s v,
+  match_stack sg s -> Val.lessdef (dummy_parent_sp s) v -> v = dummy_parent_sp s.
 Proof.
   intros. inv H0. auto. exploit parent_sp_def; eauto. tauto.
 Qed.
 
 Lemma lessdef_parent_ra:
-  forall s v,
-  match_stack s -> Val.lessdef (dummy_parent_ra s) v -> v = dummy_parent_ra s.
+  forall sg s v,
+  match_stack sg s -> Val.lessdef (dummy_parent_ra s) v -> v = dummy_parent_ra s.
 Proof.
   intros. inv H0. auto. exploit parent_ra_def; eauto. tauto.
 Qed.
